typing/pure_tcexpScript.sml
@@ -105,14 +105,15 @@ Overload subst_tc1 = ``λname v e. subst_tc (FEMPTY |+ (name,v)) e``;
 
 Definition tcexp_wf_def:
   tcexp_wf (Var v) = T ∧
-  tcexp_wf (Prim op es) = EVERY tcexp_wf es ∧
+  tcexp_wf (Prim op es) = (num_args_ok op (LENGTH es) ∧ EVERY tcexp_wf es) ∧
   tcexp_wf (App e es) = (tcexp_wf e ∧ EVERY tcexp_wf es ∧ es ≠ []) ∧
   tcexp_wf (Lam vs e) = (tcexp_wf e ∧ vs ≠ []) ∧
   tcexp_wf (Let v e1 e2) = (tcexp_wf e1 ∧ tcexp_wf e2) ∧
   tcexp_wf (Letrec fns e) = (EVERY tcexp_wf $ MAP SND fns ∧ tcexp_wf e ∧ fns ≠ []) ∧
   tcexp_wf (Case e v css) = (
     tcexp_wf e ∧ EVERY tcexp_wf $ MAP (SND o SND) css ∧
-    css ≠ [] ∧ ¬ MEM v (FLAT $ MAP (FST o SND) css)) ∧
+    css ≠ [] ∧ ¬ MEM v (FLAT $ MAP (FST o SND) css) ∧
+    ∀cn. MEM cn (MAP FST css) ⇒ cn ∉ monad_cns) ∧
   tcexp_wf (SafeProj cn ar i e) = (tcexp_wf e ∧ i < ar)
 Termination
   WF_REL_TAC `measure tcexp_size` >> rw[fetch "-" "tcexp_size_def"] >>
